{
 "cells": [
  {
   "cell_type": "markdown",
   "metadata": {},
   "source": [
    "# Intro\n",
    "Survival analysis related knowledge.\n",
    "\n",
    "## Survival function, hazard function and density function\n",
    "\n",
    "In this section we will have a brief introduction, about distribution related\n",
    "functions for survival analysis.\n",
    "\n",
    "### Definition\n",
    "In survival analysis, we view survival time T as a random variable, and we use\n",
    "the following four functions to describe it.\n",
    "\n",
    "cumulative distribution function: $$F(t) = P(T < t)$$\n",
    "\n",
    "probability density function: $$f(t) = \\frac{d{F(t)}}{dt}$$\n",
    "\n",
    "survival function: $$S(t) = 1 - F(t)$$\n",
    "\n",
    "hazard function: $$h(t) =-\\frac{\\frac{dS(t)}{dt}}{S(t)}$$\n",
    "\n",
    "cumulative hazard function: $$H(t) =\\int^t_0 h(x)dx$$\n",
    "\n",
    "### Relationship\n",
    "$$h(t) = \\frac{f(t)}{S(t)}$$\n",
    "\n",
    "$$h(t) = -\\frac{dlog(S(t))}{dt}$$\n",
    "\n",
    "$$S(t) = exp(-H(t))$$\n",
    "\n",
    "\n",
    "## Survival likelihood function\n",
    "We use $D$ to denote the cohort of objects that experienced the event (uncensored) and $D^c$ denote the cohort of objects that did not experience the event (censored). We have the likelihood function is:\n",
    "\n",
    "$$L(t) = \\prod_{i \\in D}f(t_i)\\prod_{i \\in D^c}S(t_i)=\\prod_iS(t_i) \\prod_{i \\in D}h(t_i) =\\prod_ie^{-H(t_i)} \\prod_{i \\in D}h(t_i)$$\n",
    "\n",
    "\n",
    "\n",
    "## Commonly used survival models\n",
    "### AFT (accelerated failure time model)\n",
    "#### Basic idea:\n",
    "\n",
    "$$S_1(t) = S_0(\\lambda t)$$\n",
    "\n",
    "#### A more general form:\n",
    "\n",
    "$$lnT = x\\beta + \\epsilon$$\n",
    "\n",
    "$\\epsilon$ is a random variable. The commonly used distribution for it includes Weibull and exponential.\n",
    "\n",
    "#### Prove that the genral form satisfies the basic idea:\n",
    "$$S(t) = P(T>t) = P(e^{x\\beta}e^{\\epsilon}>t) = p(Z>\\frac{t}{e^{x\\beta}}) = S_Z(\\frac{t}{e^{x\\beta}})$$\n",
    "\n",
    "$$Z = e^{\\epsilon}$$\n",
    "\n",
    "Therefore \n",
    "$$S_1(t) = S_Z(\\frac{t}{e^{x_1\\beta}}) = S_Z(\\frac{t}{e^{x_0\\beta}}\\frac{e^{x_0\\beta}}{e^{x_1\\beta}})=S_0(\\lambda t)$$\n",
    "\n",
    "#### likelihood function\n",
    "##### lemma:\n",
    "Consider $X$ has pdf $f_X(x, \\theta)$. To estimate $\\hat{\\theta}_{MLE}$ using $f_X(x, \\theta)$ and a sample $x_1, x_2, ..., x_n$ is the same as using $z_1,...z_n$ and $f_Z(z, \\theta)$, with $Z = g(X)$.\n",
    "\n",
    "##### proof:\n",
    "\n",
    "$$L(x, \\theta) = \\prod f_X(x_i, \\theta)$$\n",
    "\n",
    "$$L(z, \\theta) = \\prod f_Z(z_i,\\theta)\n",
    "= \\prod \\frac{dg^{-1}(z_i)}{dz_i}f_X(g^{-1}(z_i), \\theta) \\sim \\prod f_X(g^{-1}(z_i), \\theta) = \\prod f_X(x_i, \\theta)$$\n",
    "\n",
    "Similarly, we have \n",
    "$$S_Z(z) = P(Z>z) = P(g(X) > g(x)) = p(X>x) = S(x)$$ \n",
    "\n",
    "##### likelihood:\n",
    "\n",
    "From the above lemma we have the following survival full likelihood function, \n",
    "$$L(t) = \\prod_{i \\in D}f_T(t_i)\\prod_{i \\in D^c}S_T(t_i) \\sim \\prod_{i \\in D}f_{lnT}(ln(t_i))\\prod_{i \\in D^c}S_{lnT}(ln(t_i))$$\n",
    "\n",
    "### PH (proportional hazard)\n",
    "\n",
    "#### Basic idea:\n",
    "\n",
    "$$h_1(t) = \\lambda h_0(t)$$\n",
    "\n",
    "$$lnT = x\\beta + \\epsilon$$\n",
    "\n",
    "$\\epsilon$ is a random variable. The commonly used distribution for it includes Weibull and exponential.\n",
    "\n",
    "Prove that the genral form satisfies the basic idea:\n",
    "$$S(t) = P(T>t) = P(e^{x\\beta}e^{\\epsilon}>t) = p(Z>\\frac{t}{e^{x\\beta}}) = S_Z(\\frac{t}{e^{x\\beta}})$$\n",
    "\n",
    "$$Z = e^{\\epsilon}$$\n",
    "\n",
    "Therefore \n",
    "$$S_1(t) = S_Z(\\frac{t}{e^{x_1\\beta}}) = S_Z(\\frac{t}{e^{x_0\\beta}}\\frac{e^{x_0\\beta}}{e^{x_1\\beta}})=S_0(\\lambda t)$$\n",
    "\n",
    "\n",
    "#### likelihood function\n",
    "##### lemma:\n",
    "Consider $X$ has pdf $f_X(x, \\theta)$. To estimate $\\hat{\\theta}_{MLE}$ using $f_X(x, \\theta)$ and a sample $x_1, x_2, ..., x_n$ is the same as using $z_1,...z_n$ and $f_Z(z, \\theta)$, with $Z = g(X)$.\n",
    "\n",
    "##### proof:\n",
    "\n",
    "$$L(x, \\theta) = \\prod f_X(x_i, \\theta)$$\n",
    "\n",
    "$$L(z, \\theta) = \\prod f_Z(z_i,\\theta)\n",
    "= \\prod \\frac{dg^{-1}(z_i)}{dz_i}f_X(g^{-1}(z_i), \\theta) \\sim \\prod f_X(g^{-1}(z_i), \\theta) = \\prod f_X(x_i, \\theta)$$\n",
    "\n",
    "Similarly, we have \n",
    "$$S_Z(z) = P(Z>z) = P(g(X) > g(x)) = p(X>x) = S(x)$$ \n",
    "\n",
    "##### likelihood:\n",
    "\n",
    "From the above lemma we have the following survival full likelihood function, \n",
    "$$L(t) = \\prod_{i \\in D}f_T(t_i)\\prod_{i \\in D^c}S_T(t_i) \\sim \\prod_{i \\in D}f_{lnT}(ln(t_i))\\prod_{i \\in D^c}S_{lnT}(ln(t_i))$$\n",
    "\n",
    "### PH (proportional hazard)\n",
    "\n",
    "#### Basic idea:\n",
    "\n",
    "$$h_1(t) = \\lambda h_0(t)$$\n",
    "\n",
    "### Cox Semi-parametric proportional hazard model\n",
    "#### Basic idea\n",
    "$$h_x(t) = e^{x_i\\beta}h_0(t) = r(x_i)h_0(t)$$\n",
    "Here the $r_i$, is known as the relative risk function, which is the hazard ratio between $x_i$ and the baseline. \n",
    "\n",
    "#### partial likelihood\n",
    "Cox PH model is a semi-parametric model, in the sense that the $h_0(t)$ part (the baseline hazard function) in the hazard function is estimated in a non-parametric way. The parametric part of the likelihood function is estimated by solve the MLE of the following partial likelihood function:\n",
    "$$\\prod _j \\frac{r(x_j)}{\\sum_{i \\in R_j}r(x_i)}^{\\delta_j}$$\n",
    "\n",
    "$R_j$ is the cohort of subject at risk at time $j$, i.e, they are not censored or died yet.\n",
    "\n",
    "#### Derivation of the partial likelihood function\n",
    "https://web.stanford.edu/~lutian/coursepdf/unitcox1.pdf\n",
    "\n",
    "The full likelihood function of a PH function can be expressed as following:\n",
    "\n",
    "$$L(t) = \\prod _j e^{-H_j(t_j)} h_j(t_j)^{\\delta_j}$$\n",
    "\n",
    "$$\\delta_i = 0$$ means a case is censored; if it is 1 then otherwise.\n",
    "\n",
    "Now assuming that $$t_1 < t_2 <...< t_j$$, we then will have  \n",
    "\n",
    "$$H_j(t_j) \\approx \\sum_{i=1}^j h_j(t_i) = \\sum_{i=1}^j r(x_j)h_0(t_i)$$ (pay attention to the subscript!)\n",
    "\n",
    "The above equations lead to \n",
    "\n",
    "$$L(t) = \\prod _j e^{-H_j(t_j)} h_j(t_j)^{\\delta_j} = \\prod e^{-\\sum_{i=1}^j r(x_j)h_0(t_i)}(r(x_j)h_0(t_j))^{\\delta_j} =  \\prod e^{-\\sum_{i=1}^j r(x_j)h_i}(r(x_j)h_j)^{\\delta_j}$$\n",
    "\n",
    "And\n",
    "\n",
    "$$l(t) =\\sum_j (\\delta_j[log(r(x_j)) + log(h_j)] - \\sum_{i=1}^jr(x_j)h_i)$$\n",
    "\n",
    "The above formula of $l(t)$ can then be expressed as\n",
    "\n",
    "$$\\sum_j \\delta_j[log(r(x_j)) + log(h_j)] -\\sum_j\\sum_{i=1}^jr(x_j)h_i = \\sum_j \\delta_j[log(r(x_j)) + log(h_j)] -\\sum_jh_j\\sum_{i=j}^nr(x_i)$$\n",
    "\n",
    "By using the **profile likelihood** methodology, we can maximize $h_i$ in terms of fixed $r$, then replace $h_i$ with a function of $r$, and we will end up with the partial likelihood function."
   ]
  },
  {
   "cell_type": "code",
   "execution_count": null,
   "metadata": {},
   "outputs": [],
   "source": []
  }
 ],
 "metadata": {
  "kernelspec": {
   "display_name": "Python 3",
   "language": "python",
   "name": "python3"
  },
  "language_info": {
   "codemirror_mode": {
    "name": "ipython",
    "version": 3
   },
   "file_extension": ".py",
   "mimetype": "text/x-python",
   "name": "python",
   "nbconvert_exporter": "python",
   "pygments_lexer": "ipython3",
   "version": "3.6.5"
  }
 },
 "nbformat": 4,
 "nbformat_minor": 2
}
